SO.v
@@ -1,0 +1,658 @@
+From Coq Require Export Arith.
+Set Implicit Arguments.
+Unset Strict Implicit.
+Set Printing Projections.
+Require Import Bool.
+Require Import List.
+Require Import String.
+Require Import Coq.Lists.List Coq.Bool.Bool.
+Import Coq.Lists.List.ListNotations.
+Require Import Program.Wf.
+
+Inductive Correctness : Type :=
+| yes : Correctness
+| no : Correctness
+| trusted : Correctness
+| idk : Correctness.
+
+Inductive Node : Type :=
+  mkNode
+    {
+      content : string
+    ;correctness : Correctness
+    ; children : list Node
+    }.
+
+Inductive ComparableNode : Type :=
+  mkComparableNode
+    {
+      ComparableNodeContent : string
+    ; ComparableNodeChildren : list ComparableNode
+    }.
+
+Fixpoint get_comparable_node_from_node (n: Node) : ComparableNode :=
+  mkComparableNode (content n) (map (fun child => get_comparable_node_from_node child) (children n)).
+
+Lemma comparable_node_content_eq_to_node_content : forall n:Node, content n = ComparableNodeContent (get_comparable_node_from_node n).
+Proof.
+  intros n.
+  induction n.
+  simpl.
+  reflexivity.
+Qed.
+
+Fixpoint or_list (l : list Prop) : Prop :=
+  match l with
+    nil => False
+  | hd::tl => or hd (or_list tl)
+  end.
+
+Fixpoint is_node_in_tree (c : string) (m : Node) : Prop :=
+  or (c = content m) (or_list (map (fun child => is_node_in_tree c child) (children m))).
+
+Lemma n1_and_n2_with_same_content_and_n1_in_tree_implies_n2_in_tree : forall n1 n2 tree: Node, content n1 = content n2 /\ is_node_in_tree (content n1) tree -> is_node_in_tree (content n2) tree.
+Proof.
+  intros n1 n2 tree H.
+  intuition.
+  rewrite <- H0.
+  exact H1.
+Qed.
+
+Lemma node_is_in_itself : forall n : Node, is_node_in_tree (content n) n.
+Proof.
+  intros n.
+  induction n.
+  simpl.
+  left.
+  + reflexivity.
+Qed.
+
+Lemma head_of_non_empty_children_is_in_parent : forall parent child : Node, (children parent) <> nil /\ hd (mkNode "I don't exist"%string idk nil) (children parent) = child -> is_node_in_tree (content child) parent.
+Proof.
+  intros parent child H.
+  induction parent.
+  simpl.
+  intuition.
+  right.
+  induction children0.
+  + simpl.
+    intuition.
+  + assert (a = child).
+    intuition.
+    simpl.
+    left.
+    rewrite H.
+    apply node_is_in_itself.
+Qed.
+
+Lemma child_node_is_in_parent : forall parent child : Node, In child (children parent) -> is_node_in_tree (content child) parent.
+Proof.
+  intros parent child H.
+  induction parent.
+  simpl.
+  right.
+  induction children0.
+  + inversion H.
+  + assert (In child
+               {|
+                 content := content0;
+                 correctness := correctness0;
+                 children := a :: children0
+               |}.(children) -> child = a \/ (In child
+                                               {|
+                                                 content := content0;
+                                                 correctness := correctness0;
+                                                 children := children0
+                                               |}.(children))).
+    simpl.
+    intuition.
+    intuition.
+    rewrite <- H0.
+    simpl.
+    left.
+    apply node_is_in_itself.
+    simpl.
+    right.
+    exact H1.
+Qed.
+
+Lemma list_sum_ge_0 : forall l : list nat, 0 <= list_sum l.
+Proof.
+  intros l.
+  induction l.
+  simpl.
+  intuition.
+  simpl.
+  assert (a >= 0).
+  induction a.
+  intuition.
+  apply le_0_n.
+  subst.
+  induction a.
+  intuition.
+  intuition.
+Qed.
+
+Fixpoint and_list (l : list Prop) : Prop :=
+  match l with
+    nil => True
+  | hd::tl => and hd (and_list tl)
+  end.
+
+Lemma and_list_true_implies_element_in_list_true: forall (A : Type) (l : list A) (element : A) (x : A -> Prop), and_list (map (fun item => x item) l) /\ In element l -> x element.
+Proof.
+  intros.
+  intuition.
+  induction l.
+  + inversion H1.
+  + destruct H1.
+  - subst.
+    inversion H0.
+    exact H.
+  - inversion H0. intuition.
+Qed.
+
+Fixpoint weight (node : Node) : nat :=
+  match children node with
+    nil => 1
+  | children => S (list_sum (map (fun child => weight child) (children)))
+  end.
+
+Lemma weight_childfree_node_eq_1: forall n:Node, n.(children) = nil -> weight n = (S 0).
+Proof.
+  intros n H.
+  induction n.
+  simpl.
+  assert (children0 = nil).
+  exact H.
+  rewrite H0.
+  reflexivity.
+Qed.
+
+Lemma weight_gt_0: forall n:Node, 0 < weight n.
+Proof.
+  intros n.
+  induction n.
+  induction children0.
+  + simpl.
+    intuition.
+  + simpl.
+    intuition.
+Qed.
+
+Lemma node_weight_gt_sum_children_weight: forall n:Node, weight n > list_sum (map (fun child => weight child) (children n)).
+Proof.
+  intros n.
+  induction n.
+  simpl.
+  induction children0.
+  + simpl.
+    destruct (zerop 1).
+    discriminate.
+    exact l.
+  + simpl.
+    intuition.
+Qed.
+
+Lemma nat_in_list_le_list_sum: forall (l:list nat) (element: nat), In element l -> element <= list_sum l.
+Proof.
+  intros l element H.
+  induction l.
+  + simpl.
+    inversion H.
+  + simpl.
+    destruct H.
+  - subst.
+    apply Nat.le_add_r.
+  - transitivity (list_sum l);auto.
+    rewrite Nat.add_comm.
+    apply Nat.le_add_r.
+Qed.
+
+Lemma child_weight_le_sum_children_weight: forall (l:list Node) (child: Node), In child l -> list_sum (map (fun child => weight child) l) >= weight child.
+Proof.
+  intros l child H.
+  apply nat_in_list_le_list_sum.
+  induction l.
+  - simpl.
+    inversion H.
+  - simpl.
+    destruct H.
+    + subst.
+      intuition.
+    + subst.
+      intuition.
+Qed.
+
+Lemma parent_weight_gt_child_weight: forall parent child:Node, In child (children parent) -> weight child < weight parent.
+Proof.
+  intros parent child H.
+  induction parent.
+  simpl.
+  induction children0.
+  + inversion H.
+  + inversion H.
+  - rewrite H0.
+    intuition.
+  - intuition.
+    assert (weight child <= list_sum (map (fun child0 : Node => weight child0) children0)).
+    apply child_weight_le_sum_children_weight.
+    exact H0.
+    assert (weight a > 0).
+    apply weight_gt_0.
+    assert (weight child < (weight a + list_sum (map (fun child0 : Node => weight child0) children0))).
+    inversion H2.
+    rewrite Nat.add_comm.
+    apply Nat.lt_add_pos_r.
+    exact H3.
+    assert (weight child < S m).
+    intuition.
+    rewrite Nat.add_comm.
+    intuition.
+    intuition.
+Qed.
+
+Fixpoint are_all_idk (node : Node) : Prop :=
+  and (node.(correctness) = idk) (and_list (map (fun child => are_all_idk child) (children node))).
+
+Lemma are_all_idk_implies_children_all_idk: forall n : Node, are_all_idk n -> and_list (map (fun child => are_all_idk child) (children n)).
+Proof.
+  intros n H.
+  induction n.
+  induction children0.
+  + inversion H.
+    simpl.
+    constructor.
+  + inversion H.
+    simpl.
+    split.
+  - inversion H.
+    apply H3.
+  - apply H1.
+Qed.
+
+Definition is_debugging_tree (node : Node) : Prop :=
+  and (node.(correctness) = no) (and_list (map (fun child => are_all_idk child) (children node))).
+
+(* Lemma is_debugging_tree_true: forall node: Node, is_debugging_tree node -> and (node.(correctness) = no) (and_list (map (fun child => are_all_idk child) (children node))). *)
+(* Proof. *)
+(*   intros n H. *)
+(*   inversion H. *)
+(*   split. *)
+(*   + exact H0. *)
+(*   + exact H1. *)
+(* Qed. *)
+
+Definition get_debugging_tree_from_tree (n : Node) : Node :=
+  mkNode (content n) no (children n).
+
+Lemma debugging_tree_of_tree_has_same_weight: forall n:Node, weight n = weight (get_debugging_tree_from_tree n).
+Proof.
+  intros n.
+  induction n.
+  simpl.
+  reflexivity.
+Qed.
+
+Lemma children_of_debugging_tree_remain_unchanged: forall n:Node, children n = children (get_debugging_tree_from_tree n).
+Proof.
+  intros n.
+  induction n.
+  simpl.
+  reflexivity.
+Qed.
+
+Lemma debugging_tree_root_node_is_incorrect: forall n:Node, correctness (get_debugging_tree_from_tree n) = no.
+Proof.
+  intros n.
+  induction n.
+  simpl.
+  reflexivity.
+Qed.
+
+Lemma debugging_tree_of_tree_with_all_children_idk_is_debugging_tree: forall n:Node, and_list (map (fun child => are_all_idk child) (children n)) -> is_debugging_tree (get_debugging_tree_from_tree n).
+Proof.
+  intros n H.
+  simpl.
+  assert (children n = children (get_debugging_tree_from_tree n)).
+  apply children_of_debugging_tree_remain_unchanged.
+  assert (correctness (get_debugging_tree_from_tree n) = no).
+  apply debugging_tree_root_node_is_incorrect.
+  assert (and_list (map (fun child : Node => are_all_idk child) (get_debugging_tree_from_tree n).(children))).
+  + rewrite <- H0. exact H.
+  + unfold is_debugging_tree. split.
+  - exact H1.
+  - exact H2.
+Qed.
+Require Import Lia.
+
+Lemma debugging_tree_of_idk_tree_is_debugging_tree: forall n:Node, are_all_idk n -> is_debugging_tree (get_debugging_tree_from_tree n).
+Proof.
+  intros n H.
+  unfold is_debugging_tree.
+  split.
+  + apply debugging_tree_root_node_is_incorrect.
+  + assert (and_list (map (fun child : Node => are_all_idk child) n.(children))).
+    apply are_all_idk_implies_children_all_idk.
+  - exact H.
+  - assert (children n = children (get_debugging_tree_from_tree n)).
+    apply children_of_debugging_tree_remain_unchanged.
+    rewrite <- H1.
+    exact H0.
+Qed.
+
+Lemma comparable_node_of_debugging_tree_of_tree_is_comparable_node: forall n:Node, get_comparable_node_from_node (get_debugging_tree_from_tree n) = get_comparable_node_from_node n.
+Proof.
+  intros n.
+  induction n.
+  simpl.
+  reflexivity.
+Qed.
+
+Lemma debugging_tree_of_tree_is_in_tree: forall n:Node, is_node_in_tree (content (get_debugging_tree_from_tree n)) n.
+Proof.
+  intros n.
+  induction n.
+  simpl.
+  left.
+  reflexivity.
+Qed.
+
+Lemma content_debugging_tree_eq_content_tree: forall n:Node, content (get_debugging_tree_from_tree n) = content n.
+Proof.
+  intros n.
+  induction n.
+  simpl.
+  reflexivity.
+Qed.
+
+Obligation Tactic := intros.
+
+Program Fixpoint generic_debugging_algorithm_non_dependently_typed (n : Node) {measure (weight n)}: Node :=
+  match children n with
+    nil => n
+  | head::tail => generic_debugging_algorithm_non_dependently_typed (get_debugging_tree_from_tree head)
+  end.
+Next Obligation.
+  assert (In head (children n)).
+  + induction (children n).
+  - inversion Heq_anonymous.
+  - simpl.
+    left.
+    injection Heq_anonymous.
+    intuition.
+    + assert (weight head = weight (get_debugging_tree_from_tree head)).
+  - apply debugging_tree_of_tree_has_same_weight.
+  - rewrite <- H0.
+    apply parent_weight_gt_child_weight.
+    exact H.
+Qed.
+Next Obligation.
+  intuition.
+Qed.
+
+Obligation Tactic := Tactics.program_simpl.
+
+
+Program Fixpoint generic_debugging_algorithm_dependently_typed (n : {n: Node | is_debugging_tree n}) {measure (weight n)}: {m: Node | is_debugging_tree m /\ children m = nil} :=
+  match children n with
+    nil => n
+  | head::tail => generic_debugging_algorithm_dependently_typed (get_debugging_tree_from_tree head)
+  end.
+Next Obligation.
+  inversion H.
+  assert (are_all_idk head).
+  + assert (In head (children n)).
+  - induction (children n).
+    inversion Heq_anonymous.
+    simpl.
+    left.
+    injection Heq_anonymous.
+    intuition.
+  - apply and_list_true_implies_element_in_list_true with (children n).
+    split.
+    exact H1.
+    exact H2.
+    + apply debugging_tree_of_idk_tree_is_debugging_tree.
+      exact H2.
+Qed.
+Obligation Tactic := intros.
+Next Obligation.
+  assert (In head (children (proj1_sig n))).
+  + induction (children (proj1_sig n)).
+  - inversion Heq_anonymous.
+  - simpl.
+    left.
+    injection Heq_anonymous.
+    intuition.
+    + assert (weight head = weight (get_debugging_tree_from_tree head)).
+  - apply debugging_tree_of_tree_has_same_weight.
+  - simpl.
+    assert (match head.(children) with | [] => 1 | n0 :: l => S (weight n0 + list_sum (map (fun child : Node => weight child) l)) end = weight (get_debugging_tree_from_tree head)). intuition. rewrite H1. rewrite <- H0.
+    apply parent_weight_gt_child_weight.
+    exact H.
+Qed.
+Obligation Tactic := Tactics.program_simpl.
+
+
+Obligation Tactic := Tactics.program_simpl.
+Program Fixpoint generic_debugging_algorithm_dependently_typed3 (n : {n: Node | is_debugging_tree n}) {measure (weight n)}: {m: Node | is_debugging_tree m} :=
+  match children n with
+    nil => n
+  | head::tail => generic_debugging_algorithm_dependently_typed3 (get_debugging_tree_from_tree head)
+  end.
+
+Next Obligation.
+  apply debuggin
+Qed.
+
+Next Obligation.
+  inversion H.
+  assert (are_all_idk head).
+  + assert (In head (children n)).
+  - induction (children n).
+    inversion Heq_anonymous.
+    simpl.
+    left.
+    injection Heq_anonymous.
+    intuition.
+  - apply and_list_true_implies_element_in_list_true with (children n).
+    split.
+    exact H1.
+    exact H2.
+    + apply debugging_tree_of_idk_tree_is_debugging_tree.
+      exact H2.
+Qed.
+
+Obligation Tactic := intros.
+Next Obligation.
+  assert (In head (children (proj1_sig n))).
+  + induction (children (proj1_sig n)).
+  - inversion Heq_anonymous.
+  - simpl.
+    left.
+    injection Heq_anonymous.
+    intuition.
+    + assert (weight head = weight (get_debugging_tree_from_tree head)).
+  - apply debugging_tree_of_tree_has_same_weight.
+  - simpl.
+    assert (match head.(children) with | [] => 1 | n0 :: l => S (weight n0 + list_sum (map (fun child : Node => weight child) l)) end = weight (get_debugging_tree_from_tree head)).
+    intuition.
+    rewrite H1.
+    rewrite <- H0.
+    apply parent_weight_gt_child_weight.
+    exact H.
+Qed.
+
+Next Obligation.
+Qed.
+
+Next Obligation.
+  simpl.
+  split.
+  assert (In head (children (proj1_sig n))).
+  - induction (children (proj1_sig n)).
+    + inversion Heq_anonymous.
+    + simpl.
+      left.
+      injection Heq_anonymous.
+      intuition.
+  - assert (content (get_debugging_tree_from_tree head) = content head).
+    apply content_debugging_tree_eq_content_tree.
+    assert (is_node_in_tree (content head) (proj1_sig n)).
+    apply child_node_is_in_parent.
+    exact H.
+    inversion H0.
+    assert (content head = content (get_debugging_tree_from_tree head)).
+    apply H0.
+    simpl.
+
+    apply n1_and_n2_with_same_content_and_n1_in_tree_implies_n2_in_tree with head.
+    split.
+    + rewrite H2. intuition. simpl. auto. apply H2.
+      apply nodes_with_same_content.
+      apply
+
+
+        apply head_of_non_empty_children_is_in_parent.
+      split.
+    + intuition.
+      rewrite H0 in H.
+      inversion H.
+    + intuition.
+
+Qed.
+
+
+Program Fixpoint generic_debugging_algorithm_dependently_typed2 (n : {n: Node | is_debugging_tree n}) {measure (weight n)}: {m: Node | is_debugging_tree m /\ is_node_in_tree (content m) n} :=
+  match children n with
+    nil => n
+  | head::tail => generic_debugging_algorithm_dependently_typed2 (get_debugging_tree_from_tree head)
+  end.
+
+Next Obligation.
+  split.
+  + exact H.
+  + apply node_is_in_itself.
+Qed.
+
+Next Obligation.
+  inversion H.
+  assert (are_all_idk head).
+  + assert (In head (children n)).
+  - induction (children n).
+    inversion Heq_anonymous.
+    simpl.
+    left.
+    injection Heq_anonymous.
+    intuition.
+  - apply and_list_true_implies_element_in_list_true with (children n).
+    split.
+    exact H1.
+    exact H2.
+    + apply debugging_tree_of_idk_tree_is_debugging_tree.
+      exact H2.
+Qed.
+
+Obligation Tactic := intros.
+Next Obligation.
+  assert (In head (children (proj1_sig n))).
+  + induction (children (proj1_sig n)).
+  - inversion Heq_anonymous.
+  - simpl.
+    left.
+    injection Heq_anonymous.
+    intuition.
+    + assert (weight head = weight (get_debugging_tree_from_tree head)).
+  - apply debugging_tree_of_tree_has_same_weight.
+  - simpl.
+    assert (match head.(children) with | [] => 1 | n0 :: l => S (weight n0 + list_sum (map (fun child : Node => weight child) l)) end = weight (get_debugging_tree_from_tree head)).
+    intuition.
+    rewrite H1.
+    rewrite <- H0.
+    apply parent_weight_gt_child_weight.
+    exact H.
+Qed.
+
+Next Obligation.
+Qed.
+
+Next Obligation.
+  simpl.
+  split.
+  assert (In head (children (proj1_sig n))).
+  - induction (children (proj1_sig n)).
+    + inversion Heq_anonymous.
+    + simpl.
+      left.
+      injection Heq_anonymous.
+      intuition.
+  - assert (content (get_debugging_tree_from_tree head) = content head).
+    apply content_debugging_tree_eq_content_tree.
+    assert (is_node_in_tree (content head) (proj1_sig n)).
+    apply child_node_is_in_parent.
+    exact H.
+    inversion H0.
+    assert (content head = content (get_debugging_tree_from_tree head)).
+    apply H0.
+    simpl.
+
+    apply n1_and_n2_with_same_content_and_n1_in_tree_implies_n2_in_tree with head.
+    split.
+    + rewrite H2. intuition. simpl. auto. apply H2.
+      apply nodes_with_same_content.
+      apply
+
+
+        apply head_of_non_empty_children_is_in_parent.
+      split.
+    + intuition.
+      rewrite H0 in H.
+      inversion H.
+    + intuition.
+
+Qed.
+
+
+Fixpoint get_first_child_rec (n:Node) : Node :=
+  match children n with
+  | nil => n
+  | head::tail => get_first_child_rec head
+  end.
+
+Lemma result_node_is_in_first_child_rec : (forall n: {n:Node | is_debugging_tree n}, content (proj1_sig (generic_debugging_algorithm_dependently_typed n)) = content (get_first_child_rec (proj1_sig n))).
+  Proof.
+    intros.
+    simpl.
+    intuition.
+    induction n.
+    simpl.
+    induction x.
+    simpl.
+    intuition.
+    induction children0.
+    reflexivity.
+
+    simpl.
+    intuition.
+Lemma result_node_is_in_input_tree : (forall n: {n:Node | is_debugging_tree n}, is_node_in_tree (content (proj1_sig (generic_debugging_algorithm_dependently_typed n))) (proj1_sig n)).
+  Proof.
+    intros.
+    induction n.
+    simpl.
+    induction x.
+    induction children0.
+    + apply node_is_in_itself.
+    + simpl.
+      apply node_is_in_itself.
+
+      right.
+      simpl.
+      right.
+      simpl.
+      unfold generic_debugging_algorithm_dependently_typed.
+      simpl.
+      intuition.
+      apply node_is_in_itself.
+      intuition.
+      simpl.
